cfrontend/Ctypes.v
@@ -1506,15 +1506,15 @@ Let match_program (p: program F) (tp: program G) : Prop :=
 Theorem link_match_program:
   forall p1 p2 tp1 tp2 p,
   link p1 p2 = Some p -> match_program p1 tp1 -> match_program p2 tp2 ->
-  exists tp, link tp1 tp2 = Some tp /\ match_program p tp.
+  exists tp tp', link tp1 tp2 = Some tp /\ match_program p tp' /\ tp = tp'.
 Proof.
   intros. destruct H0, H1. 
 Local Transparent Linker_program.
   simpl in H; unfold link_program in H.
   destruct (link (program_of_program p1) (program_of_program p2)) as [pp|] eqn:LP; try discriminate.
-  assert (A: exists tpp,
+  assert (A: exists tpp tpp',
                link (program_of_program tp1) (program_of_program tp2) = Some tpp
-             /\ Linking.match_program (fun ctx f tf => match_fundef f tf) eq pp tpp).
+             /\ Linking.match_program (fun ctx f tf => match_fundef f tf) eq pp tpp' /\ tpp = tpp').
   { eapply Linking.link_match_program. 
   - intros. exploit link_match_fundef; eauto. intros (tf & A & B). exists tf; auto.
   - intros.
@@ -1525,7 +1525,7 @@ Local Transparent Linker_program.
   - eauto.
   - apply (link_linkorder _ _ _ LP).
   - apply (link_linkorder _ _ _ LP). }
-  destruct A as (tpp & TLP & MP).
+  destruct A as (tpp & tpp' & TLP & MP & EQ). subst.
   simpl; unfold link_program. rewrite TLP.
   destruct (lift_option (link (prog_types p1) (prog_types p2))) as [[typs EQ]|EQ]; try discriminate.
   destruct (link_build_composite_env (prog_types p1) (prog_types p2) typs
@@ -1538,8 +1538,10 @@ Local Transparent Linker_program.
          (prog_comp_env tp1) (prog_comp_env tp2) (prog_comp_env_eq tp1)
          (prog_comp_env_eq tp2) EQ') as (tenv & R & S).
   assert (tenv = env) by congruence. subst tenv.
-  econstructor; split; eauto. inv H. split; auto.
-  unfold program_of_program; simpl. destruct pp, tpp; exact MP.
+  inv H.
+  do 2 eexists. split; eauto. split; eauto.
+  split; auto.
+  unfold program_of_program; simpl. destruct pp, tpp'; exact MP.
 Qed.
 
 End LINK_MATCH_PROGRAM.
